spec/abstract/ARM/Arch_Structs_A.thy
@@ -323,14 +323,6 @@ definition
 where
   "arch_tcb_get_registers \<equiv> arch_tcb_context_get"
 
-text \<open>
-  This matches @{text "60 * 60 * MS_IN_S"} because it should be in micro-seconds.
-\<close>
-definition
-  MAX_SC_PERIOD :: "64 word" (* FIXME RT: Rename this to MAX_BUDGET_US to match  *)
-where
-  "MAX_SC_PERIOD \<equiv> 60 * 60 * 1000"
-
 end
 
 end
